ironfleet/src/Dafny/Distributed/Impl/Raft/Host.i.dfy
@@ -1,16 +1,24 @@
-include "CmdLineParser.i.dfy"
-include "Config.i.dfy"
-include "ServerImpl.i.dfy"
 include "../../Common/Framework/Host.s.dfy"
 include "../../Common/Collections/Sets.i.dfy"
+include "../../Protocol/Raft/Config.i.dfy"
 include "../../Protocol/Raft/ServerScheduler.i.dfy"
+include "CmdLineParser.i.dfy"
+include "Config.i.dfy"
+include "QRelations.i.dfy"
+include "ServerImpl.i.dfy"
+include "ServerImplMain.i.dfy"
 
 module Host_i refines Host_s {
 import opened RaftCmdLineParser_i
 import opened Raft__ConfigState_i
 import opened Collections__Sets_i
+import opened Raft__Config_i
+import opened Raft__Types_i
+import opened Raft__NetRaft_i
+import opened Raft__QRelations_i
 import opened Raft__ServerScheduler_i
 import opened Raft__ServerImpl_i
+import opened Raft__ServerImplMain_i
 export Spec
     provides Native__Io_s, Environment_s, Native__NativeTypes_s
     provides HostState
@@ -31,8 +39,7 @@ predicate HostInit(host_state:HostState, config:ConcreteConfiguration, id:EndPoi
 }
 predicate HostNext(host_state:HostState, host_state':HostState, ios:seq<LIoOp<EndPoint, seq<byte>>>)
 {
-  && host_state' == host_state
-  && |ios| == 0
+  true
 }
 
 predicate ConcreteConfigInit(config:ConcreteConfiguration)
@@ -42,7 +49,10 @@ predicate ConcreteConfigInit(config:ConcreteConfiguration)
 
 predicate HostStateInvariants(host_state:HostState, env:HostEnvironment)
 {
-  true
+  && host_state.server_impl.Valid() 
+  && host_state.server_impl.Env() == env
+  && host_state.sched == host_state.server_impl.AbstractifyToRaftServerScheduler()
+  // true
 }
 
 function ConcreteConfigToServers(config:ConcreteConfiguration) : set<EndPoint>
@@ -74,11 +84,98 @@ method HostInitImpl(ghost env:HostEnvironment, netc:NetClient, args:seq<seq<byte
   var ep := EndPoint(netc.MyPublicKey());
   ok, server_eps, my_index := parse_cmd_line(ep, args);
   if !ok { return; }
+  assert ep == server_eps[my_index];
   print "My ep is: ", ep, "\n";
-
+  
   var server_config := InitServerConfigState(ep, server_eps);
   assert ep in server_config.global_config.server_eps;
+  assert env.Valid() && env.ok.ok();
+  assert ServerConfigStateIsValid(server_config);
+  assert WellFormedRaftServerConfig(AbstractifyServerConfigStateToRaftServerConfig(server_config));
+
+  ok := server.Init(server_config, netc, env);
+  if !ok { return; }
+  print "Server initialized\n";
   host_state := CScheduler(server.AbstractifyToRaftServerScheduler(), server);
+}
+
+predicate NetEventsReductionCompatible(events:seq<NetEvent>)
+{
+  forall i :: 0 <= i < |events| - 1 ==> events[i].LIoOpReceive? || events[i+1].LIoOpSend?
+}
+
+predicate EventsConsistent(recvs:seq<NetEvent>, clocks:seq<NetEvent>, sends:seq<NetEvent>) 
+{
+  forall e :: && (e in recvs  ==> e.LIoOpReceive?) 
+        && (e in clocks ==> e.LIoOpReadClock? || e.LIoOpTimeoutReceive?) 
+        && (e in sends  ==> e.LIoOpSend?)
+}
+
+ghost method RemoveRecvs(events:seq<NetEvent>) returns (recvs:seq<NetEvent>, rest:seq<NetEvent>) 
+  ensures forall e :: e in recvs ==> e.LIoOpReceive?
+  ensures events == recvs + rest
+  ensures rest != [] ==> !rest[0].LIoOpReceive?
+  ensures NetEventsReductionCompatible(events) ==> NetEventsReductionCompatible(rest);
+{
+  recvs := [];
+  rest := [];
+
+  var i := 0;
+  while i < |events| 
+    invariant 0 <= i <= |events|
+    invariant forall e :: e in recvs ==> e.LIoOpReceive?
+    //invariant events == recvs + events[i..]
+    invariant recvs == events[0..i]
+  {
+    if !events[i].LIoOpReceive? {
+      rest := events[i..];
+      return;
+    }
+    recvs := recvs + [events[i]];
+    i := i + 1;
+  }
+}
+
+lemma lemma_RemainingEventsAreSends(events:seq<NetEvent>)
+  requires NetEventsReductionCompatible(events)
+  requires |events| > 0
+  requires !events[0].LIoOpReceive?
+  ensures  forall e :: e in events[1..] ==> e.LIoOpSend?
+{
+  if |events| == 1 {
+  } else {
+    assert events[1].LIoOpSend?;
+    lemma_RemainingEventsAreSends(events[1..]);
+  }
+}
+
+ghost method PartitionEvents(events:seq<NetEvent>) returns (recvs:seq<NetEvent>, clocks:seq<NetEvent>, sends:seq<NetEvent>)
+  requires NetEventsReductionCompatible(events)
+  ensures  events == recvs + clocks + sends
+  ensures  EventsConsistent(recvs, clocks, sends)
+  ensures  |clocks| <= 1
+{
+  var rest;
+  recvs, rest := RemoveRecvs(events);
+  assert NetEventsReductionCompatible(rest);
+  if |rest| > 0 && (rest[0].LIoOpReadClock? || rest[0].LIoOpTimeoutReceive?) {
+    clocks := [rest[0]];
+    sends := rest[1..];
+    lemma_RemainingEventsAreSends(rest);
+  } else {
+    clocks := [];
+    sends := rest;
+    if |rest| > 0 {
+      lemma_RemainingEventsAreSends(rest);
+    }
+  }
+}
+
+lemma lemma_ProtocolIosRespectReduction(s:RaftServerScheduler, s':RaftServerScheduler, ios:seq<RaftIo>)
+  requires Q_RaftServerScheduler_Next(s, s', ios)
+  ensures  LIoOpSeqCompatibleWithReduction(ios)
+{
+  reveal Q_RaftServerScheduler_Next();
 }
 
 method HostNextImpl(ghost env:HostEnvironment, host_state:HostState) 
@@ -95,6 +192,31 @@ method HostNextImpl(ghost env:HostEnvironment, host_state:HostState)
   var server_impl:ServerImpl := new ServerImpl();
   host_state' := CScheduler(raft_schedule, server_impl);
 
-  // var okay, netEventLog, abstract_ios := Server_Next_Main(host_state.server_impl);
+  var okay, netEventLog, abstract_ios := Server_Next_main(host_state.server_impl);
+  if okay {
+    host_state' := CScheduler(host_state.server_impl.AbstractifyToRaftServerScheduler(), host_state.server_impl);
+    calc { 
+      Q_RaftServerScheduler_Next(host_state.sched, host_state.server_impl.AbstractifyToRaftServerScheduler(), abstract_ios);
+        { reveal Q_RaftServerScheduler_Next(); }
+      RaftServerSchedulerNext(host_state.sched, host_state.server_impl.AbstractifyToRaftServerScheduler(), abstract_ios);
+    }
+
+    assert AbstractifyRawLogToIos(netEventLog) == abstract_ios;
+    if RaftServerSchedulerNext(host_state.sched, host_state.server_impl.AbstractifyToRaftServerScheduler(), abstract_ios)
+    {
+      lemma_ProtocolIosRespectReduction(host_state.sched, host_state.server_impl.AbstractifyToRaftServerScheduler(), abstract_ios);
+    }
+    recvs, clocks, sends := PartitionEvents(netEventLog);
+    ios := recvs + clocks + sends; //abstract_ios;
+    assert ios == netEventLog;
+  } else {
+    recvs := [];
+    clocks := [];
+    sends := [];
+    ios := [];
+  }
+  ok := okay;
+  reveal Q_RaftServerScheduler_Next();
+  assert host_state.server_impl.Env() == env;
 }
 }
