ironfleet/src/Dafny/Distributed/Impl/Raft/CBroadcast.i.dfy
@@ -9,10 +9,12 @@ include "PacketParsing.i.dfy"
 
 module Raft__CBroadcast_i {
 
+import opened Environment_s
 import opened Native__Io_s
 import opened Native__NativeTypes_s
 import opened Common__NetClient_i
 import opened Common__NodeIdentity_i
+import opened Concrete_NodeIdentity_i
 import opened Raft__Types_i
 import opened Raft__ConfigState_i
 import opened Raft__CMessage_i
@@ -31,5 +33,6 @@ method BuildBroadcastToEveryone(config:ConfigState, my_ep:EndPoint, msg:CMessage
 {
   broadcast := CBroadcast(my_ep, config.server_eps, msg);
 }
+
 
 }
