ironfleet/src/Dafny/Distributed/Impl/Raft/NetRaft.i.dfy
@@ -475,4 +475,5 @@ method{:timeLimitMultiplier 2} SendPacketSequence(netClient:NetClient, packets:O
 }
 
 
+
 }
