ironfleet/src/Dafny/Distributed/Impl/Raft/ServerImplDelivery.i.dfy
@@ -1,0 +1,222 @@
+include "../../Common/Collections/Seqs.i.dfy"
+include "../../../Libraries/Math/mod_auto.i.dfy"
+include "../../Protocol/Raft/Server.i.dfy"
+include "CMessage.i.dfy"
+include "CBroadcast.i.dfy"
+include "ServerImpl.i.dfy"
+include "NetRaft.i.dfy"
+include "CTypes.i.dfy"
+include "QRelations.i.dfy"
+include "PacketParsing.i.dfy"
+include "ServerImplLemmas.i.dfy"
+
+module Raft__ServerImplDelivery_i {
+
+import opened Native__Io_s
+import opened Native__NativeTypes_s
+import opened Collections__Seqs_i
+import opened Math__mod_auto_i
+import opened Raft__CMessage_i
+import opened Raft__Server_i
+import opened Raft__NetRaft_i
+import opened Raft__CTypes_i
+import opened Raft__Types_i
+import opened Raft__ServerImpl_i
+import opened Common__NodeIdentity_i
+import opened Common__NetClient_i
+import opened Common__Util_i
+import opened Environment_s
+import opened Raft__CBroadcast_i
+import opened Raft__QRelations_i
+import opened Raft__PacketParsing_i
+import opened Raft__ServerImplLemmas_i
+
+method DeliverPacket(r:ServerImpl, packets:OutboundPackets) returns (ok:bool, ghost netEventLog:seq<NetEvent>, ghost ios:seq<RaftIo>)
+  requires r.Valid()
+  requires packets.OutboundPacket?
+  requires OutboundPacketsIsValid(packets)
+  requires OutboundPacketsHasCorrectSrc(packets, r.config.server_ep)
+  modifies r.repr
+  ensures r.repr == old(r.repr)
+  ensures r.net_client != null
+  ensures ok == NetClientOk(r.net_client)
+  ensures r.Env() == old(r.Env())
+  // TOPROVE
+  // ensures r.replica == old(r.replica)
+  ensures ok ==>
+          && r.Valid()
+          && r.nextActionIndex == old(r.nextActionIndex)
+          && AllIosAreSends(ios)
+          && AbstractifyOutboundCPacketsToSeqOfRaftPackets(packets) == ExtractSentPacketsFromIos(ios)
+          && OnlySentMarshallableData(netEventLog)
+          && RawIoConsistentWithSpecIO(netEventLog, ios)
+          && old(r.Env().net.history()) + netEventLog == r.Env().net.history()
+{
+  var start_time := Time.GetDebugTimeTicks();
+  ok, netEventLog := SendPacket(r.net_client, packets, r.local_addr);
+  if (!ok) { return; }
+
+  ios := MapSentPacketToIos(packets.p);
+  lemma_MapSentPacketToIosExtractSentPacketsFromIosEquivalence(packets.p, ios);
+  var end_time := Time.GetDebugTimeTicks();
+  if packets.p.None? {
+    RecordTimingSeq("DeliverPacketEmpty", start_time, end_time);
+  } else {
+    RecordTimingSeq("DeliverPacketSingleton", start_time, end_time);
+  } 
+}
+
+method {:timeLimitMultiplier 2} DeliverPacketSequence(r:ServerImpl, packets:OutboundPackets) returns (ok:bool, ghost netEventLog:seq<NetEvent>, ghost ios:seq<RaftIo>)
+  requires r.Valid()
+  requires packets.PacketSequence?
+  requires OutboundPacketsIsValid(packets)
+  requires OutboundPacketsIsAbstractable(packets)
+  requires OutboundPacketsHasCorrectSrc(packets, r.config.server_ep)
+  modifies r.repr
+  ensures r.repr == old(r.repr)
+  ensures r.net_client != null
+  ensures ok == NetClientOk(r.net_client)
+  ensures r.Env() == old(r.Env())
+  // TOPROVE
+  // ensures r.replica == old(r.replica)
+  ensures ok ==>
+          && r.Valid()
+          && r.nextActionIndex == old(r.nextActionIndex)
+          && AllIosAreSends(ios)
+          && AbstractifyOutboundCPacketsToSeqOfRaftPackets(packets) == ExtractSentPacketsFromIos(ios)
+          && OnlySentMarshallableData(netEventLog)
+          && RawIoConsistentWithSpecIO(netEventLog, ios)
+          && old(r.Env().net.history()) + netEventLog == r.Env().net.history()
+{
+  var start_time := Time.GetDebugTimeTicks();
+  ok, netEventLog := SendPacketSequence(r.net_client, packets, r.local_addr);
+  if (!ok) { return; }
+
+  ios := MapSentPacketSeqToIos(packets.s);
+  lemma_MapSentPacketSeqToIosExtractSentPacketsFromIosEquivalence(packets, ios);
+  var end_time := Time.GetDebugTimeTicks();
+  RecordTimingSeq("DeliverPacketSequence", start_time, end_time);
+}
+
+method{:timeLimitMultiplier 2} DeliverBroadcast(r:ServerImpl, broadcast:CBroadcast) returns (ok:bool, ghost netEventLog:seq<NetEvent>, ghost ios:seq<RaftIo>)
+  requires r.Valid()
+  requires CBroadcastIsValid(broadcast)
+  requires broadcast.CBroadcast? ==> broadcast.src == r.config.server_ep;
+  modifies r.repr
+  ensures r.repr == old(r.repr)
+  ensures r.net_client != null
+  ensures ok == NetClientOk(r.net_client)
+  ensures r.Env() == old(r.Env())
+  // TOPROVE
+  // ensures r.replica == old(r.replica)
+  ensures ok ==>
+          && r.Valid()
+          && r.nextActionIndex == old(r.nextActionIndex)
+          && AllIosAreSends(ios)
+          && AbstractifyCBroadcastToRaftPacketSeq(broadcast) == ExtractSentPacketsFromIos(ios)
+          && OnlySentMarshallableData(netEventLog)
+          && RawIoConsistentWithSpecIO(netEventLog, ios)
+          && old(r.Env().net.history()) + netEventLog == r.Env().net.history()
+{
+  var start_time := Time.GetDebugTimeTicks();
+  ok, netEventLog := SendBroadcast(r.net_client, broadcast, r.local_addr);
+  if (!ok) { return; }
+
+  ios := MapBroadcastToIos(broadcast);
+  lemma_MapBroadcastToIosExtractSentPacketsFromIosEquivalence(broadcast, ios);
+    
+  lemma_NetEventLogToBroadcastRefinable(netEventLog, broadcast);
+  assert NetEventLogIsAbstractable(netEventLog);
+  if broadcast.CBroadcastNop? {
+    assert RawIoConsistentWithSpecIO(netEventLog, ios);
+  } else {
+    ghost var broadcast_ios := BuildBroadcastIos(AbstractifyEndPointToNodeIdentity(broadcast.src), 
+                                                 AbstractifyEndPointsToNodeIdentities(broadcast.dsts), 
+                                                 AbstractifyCMessageToRaftMessage(broadcast.msg));
+    calc {
+      AbstractifyRawLogToIos(netEventLog);
+      {
+        forall i | 0 <= i < |AbstractifyRawLogToIos(netEventLog)|
+          ensures AbstractifyRawLogToIos(netEventLog)[i] == 
+                    LIoOpSend(LPacket(AbstractifyEndPointsToNodeIdentities(broadcast.dsts)[i], 
+                                      AbstractifyEndPointToNodeIdentity(broadcast.src), 
+                                      AbstractifyCMessageToRaftMessage(broadcast.msg)))
+        {
+          calc {
+            AbstractifyRawLogToIos(netEventLog)[i];
+            AbstractifyNetEventToRaftIo(netEventLog[i]);
+              { lemma_NetEventLogToBroadcast(netEventLog, broadcast, i); }
+            LIoOpSend(AbstractifyCBroadcastToRaftPacketSeq(broadcast)[i]);
+            LIoOpSend(BuildLBroadcast(AbstractifyEndPointToNodeIdentity(broadcast.src), 
+                                      AbstractifyEndPointsToNodeIdentities(broadcast.dsts), 
+                                      AbstractifyCMessageToRaftMessage(broadcast.msg))[i]);
+            LIoOpSend(LPacket(AbstractifyEndPointsToNodeIdentities(broadcast.dsts)[i], 
+                              AbstractifyEndPointToNodeIdentity(broadcast.src), 
+                              AbstractifyCMessageToRaftMessage(broadcast.msg)));
+          }
+        }
+        forall i | 0 <= i < |broadcast_ios|
+          ensures broadcast_ios[i] == LIoOpSend(LPacket(AbstractifyEndPointsToNodeIdentities(broadcast.dsts)[i], 
+                                                        AbstractifyEndPointToNodeIdentity(broadcast.src), 
+                                                        AbstractifyCMessageToRaftMessage(broadcast.msg)))
+        {
+          calc {
+            LIoOpSend(LPacket(AbstractifyEndPointsToNodeIdentities(broadcast.dsts)[i], 
+                              AbstractifyEndPointToNodeIdentity(broadcast.src), 
+                              AbstractifyCMessageToRaftMessage(broadcast.msg)));
+            BuildBroadcastIos(AbstractifyEndPointToNodeIdentity(broadcast.src), 
+                              AbstractifyEndPointsToNodeIdentities(broadcast.dsts), 
+                              AbstractifyCMessageToRaftMessage(broadcast.msg))[i];
+            broadcast_ios[i];
+          }
+          }
+      }
+      broadcast_ios;
+      BuildBroadcastIos(AbstractifyEndPointToNodeIdentity(broadcast.src), 
+                        AbstractifyEndPointsToNodeIdentities(broadcast.dsts), 
+                        AbstractifyCMessageToRaftMessage(broadcast.msg));
+      MapBroadcastToIos(broadcast);
+      ios;
+    }
+    assert RawIoConsistentWithSpecIO(netEventLog, ios);
+  }
+
+  var end_time := Time.GetDebugTimeTicks();
+  if broadcast.CBroadcastNop? || (broadcast.CBroadcast? && |broadcast.dsts| as uint64 == 0) {
+    RecordTimingSeq("DeliverBroadcastEmpty", start_time, end_time);
+  } else if broadcast.CBroadcast? && |broadcast.dsts| as uint64 == 1 {
+    RecordTimingSeq("DeliverBroadcastSingleton", start_time, end_time);
+  } else {
+    RecordTimingSeq("DeliverBroadcastMany", start_time, end_time);
+  }
+}
+
+method DeliverOutboundPackets(r:ServerImpl, packets:OutboundPackets) returns (ok:bool, ghost netEventLog:seq<NetEvent>, ghost ios:seq<RaftIo>)
+  requires r.Valid()
+  requires OutboundPacketsIsValid(packets)
+  requires OutboundPacketsIsAbstractable(packets)
+  requires OutboundPacketsHasCorrectSrc(packets, r.config.server_ep);
+  modifies r.repr
+  ensures r.repr == old(r.repr)
+  ensures r.net_client != null
+  ensures ok == NetClientOk(r.net_client)
+  ensures r.Env() == old(r.Env())
+  // ensures r.replica == old(r.replica)
+  ensures ok ==>
+            &&  r.Valid()
+            && r.nextActionIndex == old(r.nextActionIndex)
+            && AllIosAreSends(ios)
+            && AbstractifyOutboundCPacketsToSeqOfRaftPackets(packets) == ExtractSentPacketsFromIos(ios)
+            && OnlySentMarshallableData(netEventLog)
+            && RawIoConsistentWithSpecIO(netEventLog, ios)
+            && OnlySentMarshallableData(netEventLog)
+            && old(r.Env().net.history()) + netEventLog == r.Env().net.history()
+{
+  match packets {
+    case Broadcast(broadcast) => ok, netEventLog, ios := DeliverBroadcast(r, broadcast);
+    case OutboundPacket(p) => ok, netEventLog, ios := DeliverPacket(r, packets);
+    case PacketSequence(s) => ok, netEventLog, ios := DeliverPacketSequence(r, packets);
+  }
+}
+
+}
