ironfleet/src/Dafny/Distributed/Impl/Raft/ServerImplLemmas.i.dfy
@@ -1,0 +1,222 @@
+include "../../Common/Collections/Seqs.i.dfy"
+include "../../Common/Framework/Environment.s.dfy"
+include "../../../Libraries/Math/mod_auto.i.dfy"
+include "../../Protocol/Raft/Server.i.dfy"
+include "ServerImpl.i.dfy"
+include "NetRaft.i.dfy"
+include "CTypes.i.dfy"
+include "CBroadcast.i.dfy"
+include "QRelations.i.dfy"
+include "CMessage.i.dfy"
+include "PacketParsing.i.dfy"
+
+module Raft__ServerImplLemmas_i {
+
+import opened Native__Io_s
+import opened Native__NativeTypes_s
+import opened Collections__Seqs_i
+import opened Math__mod_auto_i
+import opened Raft__CTypes_i
+import opened Raft__CBroadcast_i
+import opened Raft__CMessage_i
+import opened Raft__Types_i
+import opened Raft__PacketParsing_i
+import opened Raft__ServerImpl_i
+import opened Raft__Server_i
+import opened Raft__NetRaft_i
+import opened Raft__QRelations_i
+import opened Common__NodeIdentity_i
+import opened Concrete_NodeIdentity_i
+import opened Logic__Option_i
+import opened Environment_s
+
+
+function MapSentPacketToIos(sent_packet:Option<CPacket>) : seq<RaftIo>
+  requires OutboundPacketsIsValid(OutboundPacket(sent_packet))
+{
+  match sent_packet {
+    case Some(p) => [LIoOpSend(AbstractifyCPacketToRaftPacket(p))]
+    case None => []
+  }
+}
+
+lemma lemma_MapSentPacketToIosExtractSentPacketsFromIosEquivalence(sent_packet:Option<CPacket>, ios:seq<RaftIo>)
+  requires OutboundPacketsIsValid(OutboundPacket(sent_packet))
+  requires ios == MapSentPacketToIos(sent_packet)
+  ensures AbstractifyOutboundCPacketsToSeqOfRaftPackets(OutboundPacket(sent_packet)) == ExtractSentPacketsFromIos(ios)
+{
+  reveal ExtractSentPacketsFromIos();
+}
+
+function {:opaque} BuildBroadcastIos(src:NodeIdentity, dsts:seq<NodeIdentity>, msg:RaftMessage) : seq<RaftIo>
+  ensures |BuildBroadcastIos(src, dsts, msg)| == |dsts|
+  ensures forall i :: 0<=i<|dsts| ==> BuildBroadcastIos(src, dsts, msg)[i] == LIoOpSend(LPacket(dsts[i], src, msg))
+{
+  if |dsts| == 0 then []
+  else [ LIoOpSend(LPacket(dsts[0], src, msg)) ] + BuildBroadcastIos(src, dsts[1..], msg)
+}
+
+function MapBroadcastToIos(broadcast:CBroadcast) : seq<RaftIo>
+  requires CBroadcastIsAbstractable(broadcast)
+{
+  match broadcast
+    case CBroadcast(_,_,_) => BuildBroadcastIos(AbstractifyEndPointToNodeIdentity(broadcast.src), 
+                                                AbstractifyEndPointsToNodeIdentities(broadcast.dsts), 
+                                                AbstractifyCMessageToRaftMessage(broadcast.msg))
+    case CBroadcastNop => []
+}
+
+lemma lemma_NetEventLogToBroadcast(netEventLog:seq<NetEvent>, broadcast:CBroadcast, index:int)
+  requires CBroadcastIsValid(broadcast)
+  requires broadcast.CBroadcast?
+  requires 0 <= index < |netEventLog|
+  requires SendLogReflectsBroadcast(netEventLog, broadcast)
+  ensures  netEventLog[index].LIoOpSend?
+  ensures  NetPacketIsAbstractable(netEventLog[index].s)
+  ensures  AbstractifyNetPacketToRaftPacket(netEventLog[index].s) == AbstractifyCBroadcastToRaftPacketSeq(broadcast)[index]
+{
+  calc ==> {
+    true;
+    SendLogReflectsBroadcast(netEventLog, broadcast);
+    SendLogReflectsBroadcastPrefix(netEventLog, broadcast);
+    SendLogMatchesRefinement(netEventLog, broadcast, index);
+    netEventLog[index].LIoOpSend? && NetPacketIsAbstractable(netEventLog[index].s)
+      && AbstractifyCBroadcastToRaftPacketSeq(broadcast)[index] == AbstractifyNetPacketToRaftPacket(netEventLog[index].s);
+  }
+}
+
+lemma lemma_NetEventLogToBroadcastRefinable(netEventLog:seq<NetEvent>, broadcast:CBroadcast)
+  requires CBroadcastIsValid(broadcast)
+  requires SendLogReflectsBroadcast(netEventLog, broadcast)
+  ensures  NetEventLogIsAbstractable(netEventLog)
+{
+  if broadcast.CBroadcastNop? {
+    assert netEventLog == [];
+  } else {
+    forall i | 0 <= i < |netEventLog|
+      ensures NetEventIsAbstractable(netEventLog[i])
+    {
+      lemma_NetEventLogToBroadcast(netEventLog, broadcast, i);
+    }
+  }
+}
+
+lemma lemma_ExtractSentPacketsFromIos(ios:seq<RaftIo>)
+  requires AllIosAreSends(ios)
+  ensures  |ExtractSentPacketsFromIos(ios)| == |ios|
+  ensures  forall i {:auto_trigger} :: 0 <= i < |ios| ==> ExtractSentPacketsFromIos(ios)[i] == ios[i].s
+{
+  reveal ExtractSentPacketsFromIos();
+}
+
+lemma lemma_MapBroadcastToIosExtractSentPacketsFromIosEquivalence(broadcast:CBroadcast, ios:seq<RaftIo>)
+  requires CBroadcastIsAbstractable(broadcast)
+  requires ios == MapBroadcastToIos(broadcast)
+  requires AllIosAreSends(ios)
+  ensures  AbstractifyCBroadcastToRaftPacketSeq(broadcast) == ExtractSentPacketsFromIos(ios)
+{
+  reveal ExtractSentPacketsFromIos();
+
+  if broadcast.CBroadcastNop? {
+
+  } else {
+    forall i | 0 <= i < |broadcast.dsts|
+      ensures i < |ios|
+      ensures AbstractifyCBroadcastToRaftPacketSeq(broadcast)[i] == ExtractSentPacketsFromIos(ios)[i]
+    {
+      calc {
+        AbstractifyCBroadcastToRaftPacketSeq(broadcast)[i];
+        BuildLBroadcast(AbstractifyEndPointToNodeIdentity(broadcast.src), 
+                        AbstractifyEndPointsToNodeIdentities(broadcast.dsts), 
+                        AbstractifyCMessageToRaftMessage(broadcast.msg))[i];
+        LPacket(AbstractifyEndPointsToNodeIdentities(broadcast.dsts)[i], 
+                AbstractifyEndPointToNodeIdentity(broadcast.src), 
+                AbstractifyCMessageToRaftMessage(broadcast.msg));
+
+        calc {
+          LIoOpSend(LPacket(AbstractifyEndPointsToNodeIdentities(broadcast.dsts)[i], 
+                            AbstractifyEndPointToNodeIdentity(broadcast.src),
+                            AbstractifyCMessageToRaftMessage(broadcast.msg)));
+          BuildBroadcastIos(AbstractifyEndPointToNodeIdentity(broadcast.src), 
+                            AbstractifyEndPointsToNodeIdentities(broadcast.dsts), 
+                            AbstractifyCMessageToRaftMessage(broadcast.msg))[i];
+        }
+          { lemma_ExtractSentPacketsFromIos(ios); }
+        ExtractSentPacketsFromIos(BuildBroadcastIos(AbstractifyEndPointToNodeIdentity(broadcast.src), 
+                                                    AbstractifyEndPointsToNodeIdentities(broadcast.dsts), 
+                                                    AbstractifyCMessageToRaftMessage(broadcast.msg)))[i];
+        ExtractSentPacketsFromIos(ios)[i];
+      }
+    }
+
+    calc {
+      |AbstractifyCBroadcastToRaftPacketSeq(broadcast)|;
+      |broadcast.dsts|;
+      |ios|;
+        { lemma_ExtractSentPacketsFromIos(ios); }
+      |ExtractSentPacketsFromIos(ios)|;
+    }
+  }
+}
+    
+function {:opaque} MapSentPacketSeqToIos(sent_packets:seq<CPacket>) : seq<RaftIo>
+  requires OutboundPacketsIsValid(PacketSequence(sent_packets))
+  requires OutboundPacketsIsAbstractable(PacketSequence(sent_packets))
+  ensures |MapSentPacketSeqToIos(sent_packets)| == |sent_packets|
+  ensures forall i :: 0 <= i < |sent_packets| ==> MapSentPacketSeqToIos(sent_packets)[i] == LIoOpSend(AbstractifyCPacketToRaftPacket(sent_packets[i]))
+{
+  //lemma_MapSentPacketSeqToIos(sent_packets);
+  if |sent_packets| == 0 then
+  []
+  else if |sent_packets| == 1 then
+    [LIoOpSend(AbstractifyCPacketToRaftPacket(sent_packets[0]))]
+  else
+    [LIoOpSend(AbstractifyCPacketToRaftPacket(sent_packets[0]))] + MapSentPacketSeqToIos(sent_packets[1..])
+}
+lemma {:timeLimitMultiplier 3} lemma_MapSentPacketSeqToIosExtractSentPacketsFromIosEquivalence(sent_packets:OutboundPackets, ios:seq<RaftIo>)
+  requires sent_packets.PacketSequence?
+  requires OutboundPacketsIsValid(sent_packets)
+  requires OutboundPacketsIsAbstractable(sent_packets)
+  requires ios == MapSentPacketSeqToIos(sent_packets.s)
+  requires forall i :: 0 <= i < |sent_packets.s| ==> CPacketIsSendable(sent_packets.s[i])
+  ensures AbstractifyOutboundCPacketsToSeqOfRaftPackets(sent_packets) == ExtractSentPacketsFromIos(ios)
+  decreases |ios|
+{
+  assert AbstractifyOutboundCPacketsToSeqOfRaftPackets(sent_packets) == AbstractifySeqOfCPacketsToSeqOfRaftPackets(sent_packets.s);
+  reveal ExtractSentPacketsFromIos();
+  //assert |AbstractifyOutboundCPacketsToSeqOfRaftPackets(sent_packets)| == |ExtractSentPacketsFromIos(ios)|;
+  reveal MapSentPacketSeqToIos();
+  if (|ios| == 0) {
+    assert AbstractifyOutboundCPacketsToSeqOfRaftPackets(sent_packets) == ExtractSentPacketsFromIos(ios);
+  } else if (|ios| == 1) {
+    assert AbstractifyOutboundCPacketsToSeqOfRaftPackets(sent_packets) == ExtractSentPacketsFromIos(ios);
+  } else {
+    if (ios[0].LIoOpSend?) {
+      var one := ios[0];
+      var rest := PacketSequence(sent_packets.s[1..]);
+      assert ExtractSentPacketsFromIos(ios) == [ios[0].s] + ExtractSentPacketsFromIos(ios[1..]);
+            
+      lemma_MapSentPacketSeqToIosExtractSentPacketsFromIosEquivalence(rest, ios[1..]);
+      reveal AbstractifySeqOfCPacketsToSeqOfRaftPackets();
+      assert {:split_here} true;
+      calc {
+        AbstractifyOutboundCPacketsToSeqOfRaftPackets(sent_packets);
+        AbstractifySeqOfCPacketsToSeqOfRaftPackets(sent_packets.s);
+        [ios[0].s] + AbstractifyOutboundCPacketsToSeqOfRaftPackets(rest);
+        [ios[0].s] + ExtractSentPacketsFromIos(ios[1..]);
+        ExtractSentPacketsFromIos(ios);
+      }
+
+    } else {
+      assert AbstractifyOutboundCPacketsToSeqOfRaftPackets(sent_packets) == ExtractSentPacketsFromIos(ios);
+    }
+    assert AbstractifyOutboundCPacketsToSeqOfRaftPackets(sent_packets) == ExtractSentPacketsFromIos(ios);
+  }
+  //forall i | 0 <= i < |AbstractifyOutboundCPacketsToSeqOfRaftPackets(sent_packets)|
+  //    ensures AbstractifyOutboundCPacketsToSeqOfRaftPackets(sent_packets)[i] == ExtractSentPacketsFromIos(ios)[i];
+  //{
+  //}
+  assert AbstractifyOutboundCPacketsToSeqOfRaftPackets(sent_packets) == ExtractSentPacketsFromIos(ios);
+}
+
+}
