ironfleet/src/Dafny/Distributed/Impl/Raft/ServerImplNoReceiveClock.i.dfy
@@ -11,9 +11,10 @@ include "NetRaft.i.dfy"
 include "PacketParsing.i.dfy"
 include "QRelations.i.dfy"
 include "ServerImpl.i.dfy"
+include "ServerImplDelivery.i.dfy"
 // include "NetRSL.i.dfy"
 
-module Raft_ServerImplNoReceiveClock {
+module Raft__ServerImplNoReceiveClock_i {
 
 import opened Native__Io_s
 import opened Native__NativeTypes_s
@@ -30,6 +31,7 @@ import opened Raft__NetRaft_i
 import opened Raft__PacketParsing_i
 import opened Raft__QRelations_i
 import opened Raft__ServerImpl_i
+import opened Raft__ServerImplDelivery_i
 import opened Raft__Types_i
 
 method Server_Next_NoReceive_ReadClock(server_impl:ServerImpl)
@@ -37,18 +39,21 @@ method Server_Next_NoReceive_ReadClock(server_impl:ServerImpl)
   requires server_impl.nextActionIndex == 1
   requires server_impl.Valid()
   modifies server_impl.repr
-  // ensures server_impl.Repr == old(server_impl.Repr)
-  // ensures server_impl.netClient != null
-  // ensures ok == NetClientOk(server_impl.netClient)
-  // ensures server_impl.Env() == old(server_impl.Env())
-  // ensures ok ==>
-  //           && server_impl.Valid()
-  //           && server_impl.Env() == old(server_impl.Env())
-  //           && server_impl.nextActionIndex == old(server_impl.nextActionIndex)
-  //           && Q_LReplica_NoReceive_Next(old(server_impl.AbstractifyToLReplica()), server_impl.nextActionIndex as int, server_impl.AbstractifyToLReplica(), ios)
-  //           && OnlySentMarshallableData(netEventLog)
-  //           && RawIoConsistentWithSpecIO(netEventLog, ios)
-  //           && old(server_impl.Env().net.history()) + netEventLog == server_impl.Env().net.history()
+  ensures server_impl.repr == old(server_impl.repr)
+  ensures server_impl.net_client != null
+  ensures ok == NetClientOk(server_impl.net_client)
+  ensures server_impl.Env() == old(server_impl.Env())
+  ensures ok ==>
+            && server_impl.Valid()
+            && server_impl.Env() == old(server_impl.Env())
+            && server_impl.nextActionIndex == old(server_impl.nextActionIndex)
+            // TOPROVE
+            // && Q_RaftServer_NoReceive_Next(old(server_impl.AbstractifyToRaftServer()), server_impl.nextActionIndex as int, server_impl.AbstractifyToRaftServer(), ios)
+            && OnlySentMarshallableData(net_event_log)
+            && RawIoConsistentWithSpecIO(net_event_log, ios)
+            && old(server_impl.Env().net.history()) + net_event_log == server_impl.Env().net.history()
+            // TODO: can I remove?
+            && forall i :: 0 <= i < |net_event_log| - 1 ==> net_event_log[i].LIoOpReceive? || net_event_log[i+1].LIoOpSend?
 {
   ok := true;
   net_event_log := [];
@@ -57,9 +62,13 @@ method Server_Next_NoReceive_ReadClock(server_impl:ServerImpl)
   if server_impl.nextActionIndex == 1 {
     var clock,netEvent0 := ReadClock(server_impl.net_client);
     ghost var io0 := LIoOpReadClock(clock.t as int);
+    ghost var ios_head := [io0];
+    ghost var log_head := [netEvent0];
+    ghost var log_tail := [];
+    ghost var ios_tail := [];
+    ghost var preDeliveryHistory := server_impl.Env().net.history();
 
     if (server_impl.role.Leader?) {
-      ok := true;
       if (clock.t >= server_impl.next_heartbeat_time) {
         var const_params := server_impl.config.global_config.params;
         var next_heartbeat_time := UpperBoundedAdditionImpl(clock.t, const_params.heartbeat_timeout, const_params.max_integer_value);
@@ -67,16 +76,32 @@ method Server_Next_NoReceive_ReadClock(server_impl:ServerImpl)
         var msg := CMessage_AppendEntries(server_impl.current_term, server_impl.config.server_ep, 0, 0, [], 0);
         var packets := BuildBroadcastToEveryone(server_impl.config.global_config, server_impl.config.server_ep, msg);
         var packets_sent := Broadcast(packets);
-        ghost var log_tail, ios_tail;
         ok, log_tail, ios_tail := DeliverOutboundPackets(server_impl, packets_sent);
         if (!ok) { return; }
-        ghost var ios_head := [io0];
-        ghost var log_head := [netEvent0];
+        print "I broadcast heartbeat!";
         ios := ios_head + ios_tail;
         net_event_log := log_head + log_tail;
-
+        assert forall i::0<=i<|log_tail| ==> AbstractifyNetEventToRaftIo(log_tail[i]) == ios_tail[i];
+        assert forall i::0<=i<|log_tail| ==> log_tail[i].LIoOpSend? && ios_tail[i].LIoOpSend?;
+        assert forall i :: 1 <= i < |net_event_log| ==> net_event_log[i].LIoOpSend?;
+        assert forall i :: 0 <= i < |net_event_log| - 1 ==> net_event_log[i].LIoOpReceive? || net_event_log[i+1].LIoOpSend?;
       } else {
-        replica', packets_sent := ReplicaNextReadClockMaybeSendHeartbeatSkip(replica, clock);
+        net_event_log := log_head;
+        ios := ios_head;
+      }
+    } else {
+      if (clock.t >= server_impl.next_election_time) {
+        var const_params := server_impl.config.global_config.params;
+        var next_election_delta := GenerateElectionTimeout(const_params);
+        var next_election_time := UpperBoundedAdditionImpl(clock.t, next_election_delta, const_params.max_integer_value);
+        server_impl.next_election_time := next_election_time;
+        if (!ok) { return; }
+        print "My election timeout!!";
+        ios := [io0];
+        net_event_log := [netEvent0];
+      } else {
+        net_event_log := log_head;
+        ios := ios_head;
       }
     }
   }
